theories/Playground/SimTest.v
@@ -1,0 +1,89 @@
+From RSL Require Import Prelude.
+
+From stdpp Require Import strings.
+From Coinduction Require Import all.
+
+From RSL Require Import Commons.Bilogic.
+
+From RSL Require Import Simulations.FreeSim.
+
+From RSL Require Import RTL.RTL.
+From RSL Require Import RTL.Notations.
+From RSL Require Import RTL.Semantics.
+From RSL Require Import RTL.SimRules.
+
+Import RTLNotations.
+
+(* Set Mangle Names. *)
+
+Section T.
+  Let Λₜ : lang := rtl_lang.
+  Let Λₛ : lang := rtl_lang.
+  Context (Pₜ : prog Λₜ) (Pₛ : prog Λₛ).
+
+  Let n : reg := 1.
+  Let result : reg := 2.
+  Let one : reg := 3.
+  Let addr : reg := 4.
+
+  Definition fact_bad : function :=
+    {|
+      fn_name := "fact"%string;
+      fn_regs := [n; addr];
+      fn_entrypoint := 0;
+      fn_code := <{{
+            0: result := #1 -> 1;
+            1: !addr := result -> 2;
+            2: if n then goto 6 else goto 3;
+            3: result := result * n -> 4;
+            4: one := !addr -> 5;
+            5: n := n - one -> 2;
+            6: ret result;
+        }}>;
+      fn_regs_no_dup := eq_refl;
+    |}.
+
+  Definition fact_good : function :=
+    {|
+      fn_name := "fact"%string;
+      fn_regs := [n];
+      fn_entrypoint := 0;
+      fn_code := <{{
+            0: result := #1 -> 1;
+            1: one := #1 -> 2;
+            2: if n then goto 5 else goto 3;
+            3: result := result * n -> 4;
+            4: n := n - one -> 2;
+            5: ret result;
+        }}>;
+      fn_regs_no_dup := eq_refl;
+    |}.
+
+  Definition sim Φ (stepₜ: nat) '(fₜ, pcₜ) (stepₛ: nat) '(fₛ, pcₛ) : bilogic :=
+    let Φ := fun '(vₜ, mₜ) '(vₛ, mₛ) => Φ vₜ vₛ mₜ mₛ in
+    fun '(ρₜ, mₜ) '(ρₛ, mₛ) =>
+      gfp (fsim_lfp _ _ Pₜ Pₛ Φ) stepₜ ([], State fₜ pcₜ ρₜ, mₜ) stepₛ ([], State fₛ pcₛ ρₛ, mₛ).
+
+  Hint Unfold sim : custom_bilogic.
+
+  Notation "t '⟨' iₜ '≲' iₛ '⟩' s '{{' Φ '}}'" :=
+    (sim Φ iₜ t iₛ s)
+      (at level 10, no associativity).
+
+  Definition same_value (vₜ vₛ: val) (_ _: memory) :=
+    vₜ = vₛ.
+
+  Notation "(≈)" := same_value (at level 70).
+
+  Lemma inv: ∀ fuel l,
+    ⊨ one ↪ₜ 1 ->
+    addr ↪ₛ l ->
+    l →ₛ 1 ->
+    (fact_good, 2) ⟨fuel ≲ fuel⟩(fact_bad, 2) {{ (≈) }}.
+  Proof.
+    induction fuel.
+    { admit. }
+    intros l [ρₜ mₜ] [ρₛ mₛ] Hone Haddr Hl.
+    unfold_bilogic.
+  Admitted.
+End T.
