theories/RTL/SimRules.v
@@ -1,0 +1,134 @@
+From RSL Require Import Prelude.
+
+From Coinduction Require Import all.
+
+From RSL Require Import Commons.Bilogic.
+From RSL Require Import Commons.Logic.
+
+From RSL Require Import Simulations.FreeSim.
+
+From RSL Require Import RTL.RTL.
+From RSL Require Import RTL.Semantics.
+From RSL Require Import RTL.Notations.
+
+(* Set Mangle Names. *)
+
+Import RTLNotations.
+
+Section Rules.
+  Let Λₜ : lang := rtl_lang.
+  Let Λₛ : lang := rtl_lang.
+  Context (Pₜ: prog Λₜ) (Pₛ: prog Λₛ) (Φ: val -> val -> memory -> memory -> Prop).
+
+  Definition sim Φ (stepₜ: nat) '(fₜ, pcₜ) (stepₛ: nat) '(fₛ, pcₛ) : bilogic :=
+    let Φ := fun '(vₜ, mₜ) '(vₛ, mₛ) => Φ vₜ vₛ mₜ mₛ in
+    fun '(ρₜ, mₜ) '(ρₛ, mₛ) =>
+      gfp (fsim_lfp _ _ Pₜ Pₛ Φ) stepₜ ([], State fₜ pcₜ ρₜ, mₜ) stepₛ ([], State fₛ pcₛ ρₛ, mₛ).
+
+  Hint Unfold sim : custom_bilogic.
+
+  Notation "t '⟨' iₜ '≲' iₛ '⟩' s '{{' Φ '}}'" :=
+    (sim Φ iₜ t iₛ s)
+      (at level 10, no associativity).
+
+  Lemma source_nop iₜ iₛ fₜ fₛ pcₜ pcₛ : ∀ pc,
+    fₛ@pcₛ is <{ nop -> pc }> ->
+    ⊨ (fₜ, pcₜ) ⟨iₜ ≲ S iₛ⟩ (fₛ, pc) {{ Φ }} ->
+    (fₜ, pcₜ) ⟨iₜ ≲ iₛ⟩ (fₛ, pcₛ) {{ Φ }}.
+  Proof.
+    intros pc Hpc [ρₜ mₜ] [ρₛ mₛ] H.
+    unfold_bilogic.
+    apply (@fsim_roll Λₜ Λₛ).
+    eapply FSourceSteps.
+    - constructor; eassumption.
+    - eapply (@fsim_unroll Λₜ Λₛ).
+      apply H.
+  Qed.
+
+  Lemma target_nop iₜ iₛ fₜ fₛ pcₜ pcₛ : ∀ pc,
+    fₜ@pcₜ is <{ nop -> pc }> ->
+    ⊨ (fₜ, pc) ⟨S iₜ ≲ iₛ⟩ (fₛ, pcₛ) {{ Φ }} ->
+    (fₜ, pcₜ) ⟨iₜ ≲ iₛ⟩ (fₛ, pcₛ) {{ Φ }}.
+  Proof.
+    intros pc Hpc [ρₜ mₜ] [ρₛ mₛ] H.
+    unfold_bilogic.
+    apply (@fsim_roll Λₜ Λₛ).
+    eapply FTargetSteps.
+    - eexists. constructor; eassumption.
+    - intros t Hstep. inv Hstep.
+      eexists.
+      eapply (@fsim_unroll Λₜ Λₛ).
+      apply H.
+  Qed.
+
+  Lemma source_op iₜ iₛ fₜ fₛ pcₜ pcₛ :
+    ∀ pc dst op regs args v,
+    fₛ@pcₛ is <{ dst := @op regs -> pc }> ->
+    eval_op op args = Some v ->
+    ⊨ regs ↪ₛ args ->
+      ⟦ dst ↩ₛ v ⟧ (fₜ, pcₜ) ⟨iₜ ≲ S iₛ⟩ (fₛ, pc) {{ Φ }} ->
+      (fₜ, pcₜ) ⟨iₜ ≲ iₛ⟩(fₛ, pcₛ) {{ Φ }}.
+  Proof.
+    intros pc dst op regs args v Hpc Hv [ρₜ mₜ] [ρₛ mₛ].
+    intros Harg Hsim. unfold_bilogic.
+    apply (@fsim_roll Λₜ Λₛ). subst.
+    eapply FSourceSteps.
+    - econstructor; eassumption || reflexivity.
+    - eapply (@fsim_unroll Λₜ Λₛ).
+      apply Hsim.
+  Qed.
+
+  Lemma target_op iₜ iₛ fₜ fₛ pcₜ pcₛ :
+    ∀ pc dst op regs args v,
+    fₜ@pcₜ is <{ dst := @op regs -> pc }> ->
+    eval_op op args = Some v ->
+    ⊨ regs ↪ₜ args ->
+      ⟦ dst ↩ₜ v ⟧ (fₜ, pc) ⟨S iₜ ≲ iₛ⟩ (fₛ, pcₛ) {{ Φ }} ->
+      (fₜ, pcₜ) ⟨iₜ ≲ iₛ⟩(fₛ, pcₛ) {{ Φ }}.
+  Proof.
+    intros pc dst op regs args v Hpc Hv [ρₜ mₜ] [ρₛ mₛ].
+    intros Harg Hsim. unfold_bilogic.
+    apply (@fsim_roll Λₜ Λₛ). subst.
+    eapply FTargetSteps.
+    - eexists. econstructor; eassumption || reflexivity.
+    - intros t Hstep. inv Hstep.
+      eexists.
+      eapply (@fsim_unroll Λₜ Λₛ).
+      apply Hsim.
+  Qed.
+
+  Lemma source_if iₜ iₛ fₜ fₛ pcₜ pcₛ :
+    ∀ pc_true pc_false reg v,
+    fₛ@pcₛ is <{ if reg then goto pc_true else goto pc_false }> ->
+    ⊨ reg ↪ₛ v ->
+      (fₜ, pcₜ) ⟨iₜ ≲ S iₛ⟩ (fₛ, if (v =? 0)%Z then pc_true else pc_false) {{ Φ }} ->
+      (fₜ, pcₜ) ⟨iₜ ≲ iₛ⟩(fₛ, pcₛ) {{ Φ }}.
+  Proof.
+    intros pc_true pc_false reg Hpc Hv [ρₜ mₜ] [ρₛ mₛ].
+    intros Harg Hsim. unfold_bilogic.
+    apply (@fsim_roll Λₜ Λₛ). subst.
+    eapply FSourceSteps.
+    - econstructor; eassumption || reflexivity.
+    - eapply (@fsim_unroll Λₜ Λₛ).
+      apply Hsim.
+  Qed.
+
+  Lemma target_if iₜ iₛ fₜ fₛ pcₜ pcₛ :
+    ∀ pc_true pc_false reg v,
+    fₜ@pcₜ is <{ if reg then goto pc_true else goto pc_false }> ->
+    ⊨ reg ↪ₜ v ->
+      (fₜ, if (v =? 0)%Z then pc_true else pc_false) ⟨S iₜ ≲ iₛ⟩ (fₛ, pcₛ) {{ Φ }} ->
+      (fₜ, pcₜ) ⟨iₜ ≲ iₛ⟩(fₛ, pcₛ) {{ Φ }}.
+  Proof.
+    intros pc_true pc_false reg Hpc Hv [ρₜ mₜ] [ρₛ mₛ].
+    intros Harg Hsim. unfold_bilogic.
+    apply (@fsim_roll Λₜ Λₛ). subst.
+    eapply FTargetSteps.
+    - eexists. econstructor; eassumption || reflexivity.
+    - intros t Hstep. inv Hstep.
+      eexists.
+      eapply (@fsim_unroll Λₜ Λₛ).
+      apply Hsim.
+  Qed.
+
+End Rules.
