Makefile
@@ -1,0 +1,16 @@
+PROJECT = RSL
+SRC_DIR = theories
+
+.PHONY: all build check clean
+
+all: build
+
+build:
+	dune build
+
+clean:
+	dune clean
+	rm -rf _build/
+
+check: build
+	find _build/default/$(SRC_DIR) -name "*.vo" -print0 | xargs -0 rocqchk -R _build/default/$(SRC_DIR) $(PROJECT) -silent -o
